src/shim.mli
@@ -77,14 +77,14 @@ module type InterpreterType = sig
     val lookup_exported_function :
       (* string -> (store_record * Extract.instance) * Extract.module_export list -> *)
       (* config_tuple option *)
-      string -> (Dune__exe__Extract.EmptyHost.store_record * Extract.instance) *
-      Extract.module_export list ->
-      ((Dune__exe__Extract.EmptyHost.store_record * Extract.frame) * administrative_instruction list) option
+      string ->
+      (((Extract.Equality.sort * Extract.EmptyHost.store_record) * Extract.instance) * Extract.module_export list) ->
+      (((Extract.Equality.sort * Extract.EmptyHost.store_record) * Extract.frame) * Extract.administrative_instruction list) option
 
     (** Perform the instantiation of a module. *)
     val interp_instantiate_wrapper :
       Extract.module0 ->
-      (((Dune__exe__Extract.EmptyHost.store_record * Extract.instance) * Extract.module_export list) * Extract.typeidx option) option
+      ((((Extract.Equality.sort * Extract.EmptyHost.store_record) * Extract.instance) * Extract.module_export list) * Extract.nat option) option
 
     (** Parsing. *)
 
@@ -94,10 +94,10 @@ module type InterpreterType = sig
 
     val pp_values : Extract.value0 list -> string
     val pp_store : int (** The indentation level *) -> store_record -> string
-    val pp_res_tuple_except_store : res_tuple -> string
+    val pp_res_tuple_except_store :
+      ((Extract.EmptyHost.store_record * Extract.frame) * Extract.res_step) -> string
     val pp_config_tuple_except_store :
-      (* (store_record * Extract.frame) * administrative_instruction list -> *)
-      config_tuple ->
+      ((Extract.EmptyHost.store_record * Extract.frame) * Extract.administrative_instruction list) ->
       string
 
   end
